Translation/Translation.v
@@ -319,26 +319,40 @@ Definition typing_all : forall (Σ : sglobal_context)
         P (Γ,, A2) B2 (sSort s2) t0 ->
         P1 Γ (sSum n1 A1 B1) (sSum n2 A2 B2) (sSort (max_sort s1 s2))
            (XTyping.cong_Sum Σ Γ n1 n2 A1 A2 B1 B2 s1 s2 e e0 t t0)) ->
-       (forall (Γ : scontext) (n : name) (A1 A2 B1 B2 : sterm) (s1 s2 : sort)
-          (p1 p2 : sterm)
-          (e : Σ;;; Γ |-x p1 = p2 : sSum n A1 B1),
-           P1 Γ p1 p2 (sSum n A1 B1) e ->
-           forall e0 : Σ;;; Γ |-x A1 = A2 : sSort s1,
-             P1 Γ A1 A2 (sSort s1) e0 ->
-             forall e1 : Σ;;; Γ,, A1 |-x B1 = B2 : sSort s2,
-               P1 (Γ,, A1) B1 B2 (sSort s2) e1 ->
-               P1 Γ (sPi1 A1 B1 p1) (sPi1 A2 B2 p2) A1
-                  (XTyping.cong_Pi1 Σ Γ n A1 A2 B1 B2 s1 s2 p1 p2 e e0 e1)) ->
-       (forall (Γ : scontext) (n : name) (A1 A2 B1 B2 : sterm) (s1 s2 : sort)
-          (p1 p2 : sterm)
-          (e : Σ;;; Γ |-x p1 = p2 : sSum n A1 B1),
-           P1 Γ p1 p2 (sSum n A1 B1) e ->
-           forall e0 : Σ;;; Γ |-x A1 = A2 : sSort s1,
-             P1 Γ A1 A2 (sSort s1) e0 ->
-             forall e1 : Σ;;; Γ,, A1 |-x B1 = B2 : sSort s2,
-               P1 (Γ,, A1) B1 B2 (sSort s2) e1 ->
-               P1 Γ (sPi2 A1 B1 p1) (sPi2 A2 B2 p2) (B1 {0 := sPi1 A1 B1 p1})
-                  (XTyping.cong_Pi2 Σ Γ n A1 A2 B1 B2 s1 s2 p1 p2 e e0 e1)) ->
+       (forall (Γ : scontext) (nx ny : name) (A1 A2 B1 B2 : sterm) (s1 s2 : sort)
+          (p1 p2 : sterm) (e : Σ;;; Γ |-x p1 = p2 : sSum nx A1 B1),
+        P1 Γ p1 p2 (sSum nx A1 B1) e ->
+        forall e0 : Σ;;; Γ |-x A1 = A2 : sSort s1,
+        P1 Γ A1 A2 (sSort s1) e0 ->
+        forall e1 : Σ;;; Γ,, A1 |-x B1 = B2 : sSort s2,
+        P1 (Γ,, A1) B1 B2 (sSort s2) e1 ->
+        forall t : Σ;;; Γ,, A1 |-x B1 : sSort s2,
+        P (Γ,, A1) B1 (sSort s2) t ->
+        forall t0 : Σ;;; Γ,, A2 |-x B2 : sSort s2,
+        P (Γ,, A2) B2 (sSort s2) t0 ->
+        forall t1 : Σ;;; Γ |-x p1 : sSum nx A1 B1,
+        P Γ p1 (sSum nx A1 B1) t1 ->
+        forall t2 : Σ;;; Γ |-x p2 : sSum ny A2 B2,
+        P Γ p2 (sSum ny A2 B2) t2 ->
+        P1 Γ (sPi1 A1 B1 p1) (sPi1 A2 B2 p2) A1
+           (XTyping.cong_Pi1 Σ Γ nx ny A1 A2 B1 B2 s1 s2 p1 p2 e e0 e1 t t0 t1 t2)) ->
+       (forall (Γ : scontext) (nx ny : name) (A1 A2 B1 B2 : sterm) (s1 s2 : sort)
+          (p1 p2 : sterm) (e : Σ;;; Γ |-x p1 = p2 : sSum nx A1 B1),
+        P1 Γ p1 p2 (sSum nx A1 B1) e ->
+        forall e0 : Σ;;; Γ |-x A1 = A2 : sSort s1,
+        P1 Γ A1 A2 (sSort s1) e0 ->
+        forall e1 : Σ;;; Γ,, A1 |-x B1 = B2 : sSort s2,
+        P1 (Γ,, A1) B1 B2 (sSort s2) e1 ->
+        forall t : Σ;;; Γ,, A1 |-x B1 : sSort s2,
+        P (Γ,, A1) B1 (sSort s2) t ->
+        forall t0 : Σ;;; Γ,, A2 |-x B2 : sSort s2,
+        P (Γ,, A2) B2 (sSort s2) t0 ->
+        forall t1 : Σ;;; Γ |-x p1 : sSum nx A1 B1,
+        P Γ p1 (sSum nx A1 B1) t1 ->
+        forall t2 : Σ;;; Γ |-x p2 : sSum ny A2 B2,
+        P Γ p2 (sSum ny A2 B2) t2 ->
+        P1 Γ (sPi2 A1 B1 p1) (sPi2 A2 B2 p2) (B1 {0 := sPi1 A1 B1 p1})
+          (XTyping.cong_Pi2 Σ Γ nx ny A1 A2 B1 B2 s1 s2 p1 p2 e e0 e1 t t0 t1 t2)) ->
        (forall (Γ : scontext) (s : sort) (A1 A2 u1 u2 v1 v2 : sterm)
           (e : Σ;;; Γ |-x A1 = A2 : sSort s),
         P1 Γ A1 A2 (sSort s) e ->
@@ -537,7 +551,75 @@ Proof.
       now apply trans_Sum.
 
     (* type_Pi1 *)
-    + fail "todo".
+    + (* Translation of the domain *)
+      destruct (H0 _ hΓ) as [S' [A'' hA'']].
+      assert (th : type_head (head (sSort s1))) by constructor.
+      destruct (choose_type hg th hA'') as [T' [[A' hA'] hh]].
+      clear hA'' A'' S'.
+      destruct T' ; inversion hh.
+      subst. clear hh th.
+      (* Translation of the codomain *)
+      destruct (H1 _ (trans_snoc hΓ hA'))
+        as [S' [B'' hB'']].
+      assert (th : type_head (head (sSort s2))) by constructor.
+      destruct (choose_type hg th hB'') as [T' [[B' hB'] hh]].
+      clear hB'' B'' S'.
+      destruct T' ; inversion hh. subst. clear hh th.
+      (* Translation of the pair *)
+      destruct (H _ hΓ) as [T'' [p'' hp'']].
+      assert (th : type_head (head (sSum n A B))) by constructor.
+      destruct (choose_type hg th hp'') as [T' [[p' hp'] hh]].
+      clear hp'' p'' T''.
+      destruct T' ; inversion hh. subst. clear hh th.
+      rename T'1 into A'', T'2 into B''.
+      destruct (change_type hg hp' (trans_Sum hΓ hA' hB')) as [p'' hp''].
+      clear hp' A'' B'' p'.
+    (* Now we conclude *)
+      exists A', (sPi1 A' B' p'').
+      destruct hp'' as [[[? ?] ?] hp'].
+      destruct hA' as [[[? ?] ?] hA'].
+      destruct hB' as [[[? ?] ?] hB'].
+      repeat split.
+      * assumption.
+      * assumption.
+      * constructor ; assumption.
+      * eapply type_Pi1' ; eassumption.
+
+    (* type_Pi2 *)
+    + (* Translation of the domain *)
+      destruct (H0 _ hΓ) as [S' [A'' hA'']].
+      assert (th : type_head (head (sSort s1))) by constructor.
+      destruct (choose_type hg th hA'') as [T' [[A' hA'] hh]].
+      clear hA'' A'' S'.
+      destruct T' ; inversion hh.
+      subst. clear hh th.
+      (* Translation of the codomain *)
+      destruct (H1 _ (trans_snoc hΓ hA'))
+        as [S' [B'' hB'']].
+      assert (th : type_head (head (sSort s2))) by constructor.
+      destruct (choose_type hg th hB'') as [T' [[B' hB'] hh]].
+      clear hB'' B'' S'.
+      destruct T' ; inversion hh. subst. clear hh th.
+      (* Translation of the pair *)
+      destruct (H _ hΓ) as [T'' [p'' hp'']].
+      assert (th : type_head (head (sSum n A B))) by constructor.
+      destruct (choose_type hg th hp'') as [T' [[p' hp'] hh]].
+      clear hp'' p'' T''.
+      destruct T' ; inversion hh. subst. clear hh th.
+      rename T'1 into A'', T'2 into B''.
+      destruct (change_type hg hp' (trans_Sum hΓ hA' hB')) as [p'' hp''].
+      clear hp' A'' B'' p'.
+    (* Now we conclude *)
+      exists (B'{ 0 := sPi1 A' B' p'' }), (sPi2 A' B' p'').
+      destruct hp'' as [[[? ?] ?] hp'].
+      destruct hA' as [[[? ?] ?] hA'].
+      destruct hB' as [[[? ?] ?] hB'].
+      repeat split.
+      * assumption.
+      * apply inrel_subst ; try assumption.
+        constructor ; assumption.
+      * constructor ; assumption.
+      * eapply type_Pi2' ; eassumption.
 
     (* type_Eq *)
     + (* The type *)
@@ -1723,6 +1805,477 @@ Proof.
       cbn in hp5. rewrite <- llift_substProj, <- rlift_substProj in hp5.
       rewrite !llift00, !rlift00 in hp5.
       apply hp5.
+
+    (* cong_Pi1 *)
+    + (* The domains *)
+      destruct (H0 _ hΓ)
+        as [T1 [T2 [A1'' [A2'' [pA h1']]]]].
+      destruct (eqtrans_trans hg h1') as [hA1'' hA2''].
+      destruct h1' as [[[[[? ?] ?] ?] ?] hpA''].
+      assert (th : type_head (head (sSort s1))) by constructor.
+      destruct (choose_type hg th hA1'') as [T' [[A1' hA1'] hh]].
+      destruct T' ; inversion hh. subst.
+      clear hh.
+      destruct (choose_type hg th hA2'') as [T' [[A2' hA2'] hh]].
+      destruct T' ; inversion hh. subst.
+      clear hh th.
+      (* Now the codomains *)
+      destruct (H1 _ (trans_snoc hΓ hA1'))
+        as [S1 [S2 [B1'' [B2'' [pB h2']]]]].
+      destruct (eqtrans_trans hg h2') as [hB1'' hB2''].
+      assert (th : type_head (head (sSort s2))) by constructor.
+      destruct (choose_type hg th hB1'') as [T' [[B1' hB1'] hh]].
+      destruct T' ; inversion hh. subst.
+      clear hh.
+      destruct (choose_type hg th hB2'') as [T' [[B2' hB2'] hh]].
+      destruct T' ; inversion hh. subst.
+      clear hh th.
+      destruct h2' as [[[[[? ?] ?] ?] ?] hpB''].
+      (* Now we connect the paths for the domains *)
+      assert (hq1 : ∑ p1, Σ ;;; Γ' |-i p1 : sHeq (sSort s1) A1' (sSort s1) A2').
+      { destruct hA1' as [[_ eA1'] hA1'].
+        destruct hA1'' as [_ hA1''].
+        destruct hA2' as [[_ eA2'] hA2'].
+        destruct hA2'' as [_ hA2''].
+        assert (hr : A1' ∼ A1'').
+        { eapply trel_trans.
+          - eapply trel_sym. eapply inrel_trel. eassumption.
+          - eapply inrel_trel. eassumption.
+        }
+        destruct (trel_to_heq Γ' hg hr) as [pl hpl].
+        specialize (hpl _ _ ltac:(eassumption) ltac:(eassumption)).
+        assert (hr' : A2'' ∼ A2').
+        { eapply trel_trans.
+          - eapply trel_sym. eapply inrel_trel. eassumption.
+          - eapply inrel_trel. eassumption.
+        }
+        destruct (trel_to_heq Γ' hg hr') as [pr hpr].
+        specialize (hpr _ _ ltac:(eassumption) ltac:(eassumption)).
+        exists (sHeqTrans (sHeqTrans pl pA) pr).
+        eapply type_HeqTrans' ; try assumption.
+        - eapply type_HeqTrans' ; eassumption.
+        - eassumption.
+      }
+      destruct hq1 as [q1 hq1].
+      (* And then the paths for the codomains *)
+      pose (Γ1 := nil ,, A1').
+      pose (Γ2 := nil ,, A2').
+      pose (Γm := [ sPack A1' A2' ]).
+      assert (hm : ismix Σ Γ' Γ1 Γ2 Γm).
+      { revert Γm.
+        replace A1' with (llift0 #|@nil sterm| A1')
+          by (cbn ; now rewrite llift00).
+        replace A2' with (rlift0 #|@nil sterm| A2')
+          by (cbn ; now rewrite rlift00).
+        intros.
+        destruct hA1' as [[? ?] ?].
+        destruct hA2' as [[? ?] ?].
+        econstructor.
+        - constructor.
+        - eassumption.
+        - assumption.
+      }
+      pose (Δ := Γ' ,,, Γm).
+      assert (hq2 : ∑ q2, Σ ;;; Γ' ,,, Γ1 |-i q2 : sHeq (sSort s2) B1'
+                                                       (sSort s2) B2').
+      { destruct hB1' as [[_ eB1'] hB1'].
+        destruct hB1'' as [_ hB1''].
+        destruct hB2' as [[_ eB2'] hB2'].
+        destruct hB2'' as [_ hB2''].
+        assert (hr : B1' ∼ B1'').
+        { eapply trel_trans.
+          - eapply trel_sym. eapply inrel_trel. eassumption.
+          - eapply inrel_trel. eassumption.
+        }
+        destruct (trel_to_heq (Γ',, A1') hg hr) as [pl hpl].
+        specialize (hpl _ _ ltac:(eassumption) ltac:(eassumption)).
+        assert (hr' : B2'' ∼ B2').
+        { eapply trel_trans.
+          - eapply trel_sym. eapply inrel_trel. eassumption.
+          - eapply inrel_trel. eassumption.
+        }
+        destruct (trel_to_heq (Γ',, A1') hg hr') as [pr hpr].
+        specialize (hpr _ _ ltac:(eassumption) ltac:(eassumption)).
+        exists (sHeqTrans (sHeqTrans pl pB) pr).
+        eapply type_HeqTrans' ; try assumption.
+        - eapply type_HeqTrans' ; eassumption.
+        - eassumption.
+      }
+      destruct hq2 as [q2 hq2].
+      assert (hp3 : ∑ p3, Σ ;;; Δ |-i p3 : sHeq (sSort s2)
+                                               (llift0 #|Γm| B1')
+                                               (sSort s2)
+                                               (llift0 #|Γm| B2')
+             ).
+      { exists (llift0 #|Γm| q2).
+        match goal with
+        | |- _ ;;; _ |-i _ : ?T =>
+          change T with (llift0 #|Γm| (sHeq (sSort s2) B1' (sSort s2) B2'))
+        end.
+        eapply type_llift0 ; try easy.
+      }
+      destruct hp3 as [p3 hp3].
+      (* Also translating the typing hypothesis for B2 *)
+      destruct (H3 _ (trans_snoc hΓ hA2'))
+        as [S' [B2''' hB2''']].
+      assert (th : type_head (head (sSort s2))) by constructor.
+      destruct (choose_type hg th hB2''') as [T' [[tB2 htB2] hh]].
+      clear hB2''' B2''' S'.
+      destruct T' ; inversion hh. subst. clear hh th.
+      (* Now we can use the strong version of the lemma to build a path between
+         B2' and tB2 !
+       *)
+      assert (hp4 : ∑ p4, Σ ;;; Δ |-i p4 : sHeq (sSort s2) (llift0 #|Γm| B2')
+                                               (sSort s2) (rlift0 #|Γm| tB2)
+             ).
+      { change (sSort s2) with (llift0 #|Γm| (sSort s2)) at 1.
+        change (sSort s2) with (rlift0 #|Γm| (sSort s2)) at 2.
+        assert (hr : B2' ∼ tB2).
+        { destruct htB2 as [[? ?] ?].
+          destruct hB2' as [[? ?] ?].
+          eapply trel_trans.
+          + eapply trel_sym. eapply inrel_trel. eassumption.
+          + apply inrel_trel. assumption.
+        }
+        edestruct (trel_to_heq' hg hr) as [p4 hp4].
+        exists p4. apply hp4.
+        - eassumption.
+        - destruct hB2' as [[? ?] ?]. assumption.
+        - destruct htB2 as [[? ?] ?]. assumption.
+      }
+      destruct hp4 as [p4 hp4].
+      (* This gives us a better path *)
+      assert (hp5 : ∑ p5, Σ ;;; Δ |-i p5 : sHeq (sSort s2) (llift0 #|Γm| B1')
+                                               (sSort s2) (rlift0 #|Γm| tB2)
+             ).
+      { exists (sHeqTrans p3 p4).
+        eapply type_HeqTrans' ; eassumption.
+      }
+      destruct hp5 as [p5 hp5].
+      (* Cleaning *)
+      clear hp4 p4 hp3 p3 hq2 q2.
+      clear hB2' B2' hB2'' hpB'' hB1'' hpA'' hA1'' hA2''.
+      (* clear i8 i7 i6 i5 i4 S1 S2 B1'' B2'' pB. *)
+      (* clear i3 i2 i1 i0 i T1 T2 A1'' A2'' pA. *)
+      clear pA pB pi2_1 pi2_2 A1'' A2''.
+      rename q1 into pA, p5 into pB, hq1 into hpA, hp5 into hpB.
+      rename tB2 into B2', htB2 into hB2'.
+      (* We can now translate the pairs. *)
+      destruct (H _ hΓ)
+        as [P1 [P1' [p1'' [p2'' [pt h3']]]]].
+      destruct (eqtrans_trans hg h3') as [hp1'' hp2''].
+      destruct (change_type hg hp1'' (trans_Sum hΓ hA1' hB1')) as [p1' hp1'].
+      destruct (change_type hg hp2'' (trans_Sum hΓ hA1' hB1')) as [p2' hp2'].
+      destruct h3' as [[[[[? ?] ?] ?] ?] hpt].
+      destruct (H5 _ hΓ)
+        as [P2 [p2''' hp2''']].
+      destruct (change_type hg hp2''' (trans_Sum hΓ hA2' hB2')) as [tp2 htp2].
+      clear hp2''' p2''' P2.
+      assert (hqt : ∑ qt,
+        Σ ;;; Γ' |-i qt : sHeq (sSum nx A1' B1') p1' (sSum ny A2' B2') tp2
+      ).
+      { destruct hp1'' as [[[? ?] ?] ?].
+        destruct hp2'' as [[[? ?] ?] ?].
+        destruct hp1' as [[[? ?] ?] ?].
+        destruct hp2' as [[[? ?] ?] ?].
+        destruct htp2 as [[[? ?] ?] ?].
+        assert (r1 : p1' ∼ p1'').
+        { eapply trel_trans.
+          - eapply trel_sym. eapply inrel_trel. eassumption.
+          - apply inrel_trel. assumption.
+        }
+        destruct (trel_to_heq Γ' hg r1) as [pl hpl].
+        specialize (hpl _ _ ltac:(eassumption) ltac:(eassumption)).
+        assert (r2 : p2'' ∼ tp2).
+        { eapply trel_trans.
+          - eapply trel_sym. eapply inrel_trel. eassumption.
+          - apply inrel_trel. assumption.
+        }
+        destruct (trel_to_heq Γ' hg r2) as [pr hpr].
+        specialize (hpr _ _ ltac:(eassumption) ltac:(eassumption)).
+        exists (sHeqTrans pl (sHeqTrans pt pr)).
+        eapply type_HeqTrans' ; try assumption.
+        - eassumption.
+        - eapply type_HeqTrans' ; eassumption.
+      }
+      destruct hqt as [qt hqt].
+      (* We have an equality between Pi1s now *)
+      assert (hpi : ∑ qpi,
+        Σ ;;; Γ' |-i qpi : sHeq A1' (sPi1 A1' B1' p1')
+                               A2' (sPi1 A2' B2' tp2)
+      ).
+      { exists (sCongPi1 B1' B2' pA pB qt).
+        destruct hB1' as [[[? ?] ?] ?].
+        destruct hB2' as [[[? ?] ?] ?].
+        eapply type_CongPi1' ; try eassumption.
+        cbn in hpB. rewrite <- llift_substProj, <- rlift_substProj in hpB.
+        rewrite !llift00, !rlift00 in hpB.
+        apply hpB.
+      }
+      destruct hpi as [qpi hpi].
+      (* Finally we translate the right Pi1 to put it in the left Sum *)
+      rename e into eA.
+      pose (e := sHeqTypeEq A2' A1' (sHeqSym qpi)).
+      pose (tpi := sTransport A2' A1' e (sPi1 A2' B2' tp2)).
+      (* We conclude *)
+      exists A1', A1'.
+      exists (sPi1 A1' B1' p1'), tpi.
+      exists (sHeqTrans qpi (sHeqTransport e (sPi1 A2' B2' tp2))).
+      destruct hp1' as [[[? ?] ?] ?].
+      destruct htp2 as [[[? ?] ?] ?].
+      destruct hA1' as [[[? ?] ?] ?].
+      destruct hA2' as [[[? ?] ?] ?].
+      destruct hB1' as [[[? ?] ?] ?].
+      destruct hB2' as [[[? ?] ?] ?].
+      repeat split.
+      * assumption.
+      * assumption.
+      * assumption.
+      * constructor ; assumption.
+      * constructor. constructor ; assumption.
+      * eapply type_HeqTrans' ; try eassumption.
+        eapply type_HeqTransport' ; try assumption.
+        -- eapply type_Pi1' ; eassumption.
+        -- eapply type_HeqTypeEq' ; try assumption.
+           ++ eapply type_HeqSym' ; eassumption.
+           ++ eassumption.
+
+    (* cong_Pi2 *)
+    + (* The domains *)
+      destruct (H0 _ hΓ)
+        as [T1 [T2 [A1'' [A2'' [pA h1']]]]].
+      destruct (eqtrans_trans hg h1') as [hA1'' hA2''].
+      destruct h1' as [[[[[? ?] ?] ?] ?] hpA''].
+      assert (th : type_head (head (sSort s1))) by constructor.
+      destruct (choose_type hg th hA1'') as [T' [[A1' hA1'] hh]].
+      destruct T' ; inversion hh. subst.
+      clear hh.
+      destruct (choose_type hg th hA2'') as [T' [[A2' hA2'] hh]].
+      destruct T' ; inversion hh. subst.
+      clear hh th.
+      (* Now the codomains *)
+      destruct (H1 _ (trans_snoc hΓ hA1'))
+        as [S1 [S2 [B1'' [B2'' [pB h2']]]]].
+      destruct (eqtrans_trans hg h2') as [hB1'' hB2''].
+      assert (th : type_head (head (sSort s2))) by constructor.
+      destruct (choose_type hg th hB1'') as [T' [[B1' hB1'] hh]].
+      destruct T' ; inversion hh. subst.
+      clear hh.
+      destruct (choose_type hg th hB2'') as [T' [[B2' hB2'] hh]].
+      destruct T' ; inversion hh. subst.
+      clear hh th.
+      destruct h2' as [[[[[? ?] ?] ?] ?] hpB''].
+      (* Now we connect the paths for the domains *)
+      assert (hq1 : ∑ p1, Σ ;;; Γ' |-i p1 : sHeq (sSort s1) A1' (sSort s1) A2').
+      { destruct hA1' as [[_ eA1'] hA1'].
+        destruct hA1'' as [_ hA1''].
+        destruct hA2' as [[_ eA2'] hA2'].
+        destruct hA2'' as [_ hA2''].
+        assert (hr : A1' ∼ A1'').
+        { eapply trel_trans.
+          - eapply trel_sym. eapply inrel_trel. eassumption.
+          - eapply inrel_trel. eassumption.
+        }
+        destruct (trel_to_heq Γ' hg hr) as [pl hpl].
+        specialize (hpl _ _ ltac:(eassumption) ltac:(eassumption)).
+        assert (hr' : A2'' ∼ A2').
+        { eapply trel_trans.
+          - eapply trel_sym. eapply inrel_trel. eassumption.
+          - eapply inrel_trel. eassumption.
+        }
+        destruct (trel_to_heq Γ' hg hr') as [pr hpr].
+        specialize (hpr _ _ ltac:(eassumption) ltac:(eassumption)).
+        exists (sHeqTrans (sHeqTrans pl pA) pr).
+        eapply type_HeqTrans' ; try assumption.
+        - eapply type_HeqTrans' ; eassumption.
+        - eassumption.
+      }
+      destruct hq1 as [q1 hq1].
+      (* And then the paths for the codomains *)
+      pose (Γ1 := nil ,, A1').
+      pose (Γ2 := nil ,, A2').
+      pose (Γm := [ sPack A1' A2' ]).
+      assert (hm : ismix Σ Γ' Γ1 Γ2 Γm).
+      { revert Γm.
+        replace A1' with (llift0 #|@nil sterm| A1')
+          by (cbn ; now rewrite llift00).
+        replace A2' with (rlift0 #|@nil sterm| A2')
+          by (cbn ; now rewrite rlift00).
+        intros.
+        destruct hA1' as [[? ?] ?].
+        destruct hA2' as [[? ?] ?].
+        econstructor.
+        - constructor.
+        - eassumption.
+        - assumption.
+      }
+      pose (Δ := Γ' ,,, Γm).
+      assert (hq2 : ∑ q2, Σ ;;; Γ' ,,, Γ1 |-i q2 : sHeq (sSort s2) B1'
+                                                       (sSort s2) B2').
+      { destruct hB1' as [[_ eB1'] hB1'].
+        destruct hB1'' as [_ hB1''].
+        destruct hB2' as [[_ eB2'] hB2'].
+        destruct hB2'' as [_ hB2''].
+        assert (hr : B1' ∼ B1'').
+        { eapply trel_trans.
+          - eapply trel_sym. eapply inrel_trel. eassumption.
+          - eapply inrel_trel. eassumption.
+        }
+        destruct (trel_to_heq (Γ',, A1') hg hr) as [pl hpl].
+        specialize (hpl _ _ ltac:(eassumption) ltac:(eassumption)).
+        assert (hr' : B2'' ∼ B2').
+        { eapply trel_trans.
+          - eapply trel_sym. eapply inrel_trel. eassumption.
+          - eapply inrel_trel. eassumption.
+        }
+        destruct (trel_to_heq (Γ',, A1') hg hr') as [pr hpr].
+        specialize (hpr _ _ ltac:(eassumption) ltac:(eassumption)).
+        exists (sHeqTrans (sHeqTrans pl pB) pr).
+        eapply type_HeqTrans' ; try assumption.
+        - eapply type_HeqTrans' ; eassumption.
+        - eassumption.
+      }
+      destruct hq2 as [q2 hq2].
+      assert (hp3 : ∑ p3, Σ ;;; Δ |-i p3 : sHeq (sSort s2)
+                                               (llift0 #|Γm| B1')
+                                               (sSort s2)
+                                               (llift0 #|Γm| B2')
+             ).
+      { exists (llift0 #|Γm| q2).
+        match goal with
+        | |- _ ;;; _ |-i _ : ?T =>
+          change T with (llift0 #|Γm| (sHeq (sSort s2) B1' (sSort s2) B2'))
+        end.
+        eapply type_llift0 ; try easy.
+      }
+      destruct hp3 as [p3 hp3].
+      (* Also translating the typing hypothesis for B2 *)
+      destruct (H3 _ (trans_snoc hΓ hA2'))
+        as [S' [B2''' hB2''']].
+      assert (th : type_head (head (sSort s2))) by constructor.
+      destruct (choose_type hg th hB2''') as [T' [[tB2 htB2] hh]].
+      clear hB2''' B2''' S'.
+      destruct T' ; inversion hh. subst. clear hh th.
+      (* Now we can use the strong version of the lemma to build a path between
+         B2' and tB2 !
+       *)
+      assert (hp4 : ∑ p4, Σ ;;; Δ |-i p4 : sHeq (sSort s2) (llift0 #|Γm| B2')
+                                               (sSort s2) (rlift0 #|Γm| tB2)
+             ).
+      { change (sSort s2) with (llift0 #|Γm| (sSort s2)) at 1.
+        change (sSort s2) with (rlift0 #|Γm| (sSort s2)) at 2.
+        assert (hr : B2' ∼ tB2).
+        { destruct htB2 as [[? ?] ?].
+          destruct hB2' as [[? ?] ?].
+          eapply trel_trans.
+          + eapply trel_sym. eapply inrel_trel. eassumption.
+          + apply inrel_trel. assumption.
+        }
+        edestruct (trel_to_heq' hg hr) as [p4 hp4].
+        exists p4. apply hp4.
+        - eassumption.
+        - destruct hB2' as [[? ?] ?]. assumption.
+        - destruct htB2 as [[? ?] ?]. assumption.
+      }
+      destruct hp4 as [p4 hp4].
+      (* This gives us a better path *)
+      assert (hp5 : ∑ p5, Σ ;;; Δ |-i p5 : sHeq (sSort s2) (llift0 #|Γm| B1')
+                                               (sSort s2) (rlift0 #|Γm| tB2)
+             ).
+      { exists (sHeqTrans p3 p4).
+        eapply type_HeqTrans' ; eassumption.
+      }
+      destruct hp5 as [p5 hp5].
+      (* Cleaning *)
+      clear hp4 p4 hp3 p3 hq2 q2.
+      clear hB2' B2' hB2'' hpB'' hB1'' hpA'' hA1'' hA2''.
+      (* clear i8 i7 i6 i5 i4 S1 S2 B1'' B2'' pB. *)
+      (* clear i3 i2 i1 i0 i T1 T2 A1'' A2'' pA. *)
+      clear pA pB pi2_1 pi2_2 A1'' A2''.
+      rename q1 into pA, p5 into pB, hq1 into hpA, hp5 into hpB.
+      rename tB2 into B2', htB2 into hB2'.
+      (* We can now translate the pairs. *)
+      destruct (H _ hΓ)
+        as [P1 [P1' [p1'' [p2'' [pt h3']]]]].
+      destruct (eqtrans_trans hg h3') as [hp1'' hp2''].
+      destruct (change_type hg hp1'' (trans_Sum hΓ hA1' hB1')) as [p1' hp1'].
+      destruct (change_type hg hp2'' (trans_Sum hΓ hA1' hB1')) as [p2' hp2'].
+      destruct h3' as [[[[[? ?] ?] ?] ?] hpt].
+      destruct (H5 _ hΓ)
+        as [P2 [p2''' hp2''']].
+      destruct (change_type hg hp2''' (trans_Sum hΓ hA2' hB2')) as [tp2 htp2].
+      clear hp2''' p2''' P2.
+      assert (hqt : ∑ qt,
+        Σ ;;; Γ' |-i qt : sHeq (sSum nx A1' B1') p1' (sSum ny A2' B2') tp2
+      ).
+      { destruct hp1'' as [[[? ?] ?] ?].
+        destruct hp2'' as [[[? ?] ?] ?].
+        destruct hp1' as [[[? ?] ?] ?].
+        destruct hp2' as [[[? ?] ?] ?].
+        destruct htp2 as [[[? ?] ?] ?].
+        assert (r1 : p1' ∼ p1'').
+        { eapply trel_trans.
+          - eapply trel_sym. eapply inrel_trel. eassumption.
+          - apply inrel_trel. assumption.
+        }
+        destruct (trel_to_heq Γ' hg r1) as [pl hpl].
+        specialize (hpl _ _ ltac:(eassumption) ltac:(eassumption)).
+        assert (r2 : p2'' ∼ tp2).
+        { eapply trel_trans.
+          - eapply trel_sym. eapply inrel_trel. eassumption.
+          - apply inrel_trel. assumption.
+        }
+        destruct (trel_to_heq Γ' hg r2) as [pr hpr].
+        specialize (hpr _ _ ltac:(eassumption) ltac:(eassumption)).
+        exists (sHeqTrans pl (sHeqTrans pt pr)).
+        eapply type_HeqTrans' ; try assumption.
+        - eassumption.
+        - eapply type_HeqTrans' ; eassumption.
+      }
+      destruct hqt as [qt hqt].
+      (* We have an equality between Pi1s now *)
+      assert (hpi : ∑ qpi,
+        Σ ;;; Γ' |-i qpi : sHeq (B1'{ 0 := sPi1 A1' B1' p1' }) (sPi2 A1' B1' p1')
+                               (B2'{ 0 := sPi1 A2' B2' tp2 }) (sPi2 A2' B2' tp2)
+      ).
+      { exists (sCongPi2 B1' B2' pA pB qt).
+        destruct hB1' as [[[? ?] ?] ?].
+        destruct hB2' as [[[? ?] ?] ?].
+        eapply type_CongPi2' ; try eassumption.
+        cbn in hpB. rewrite <- llift_substProj, <- rlift_substProj in hpB.
+        rewrite !llift00, !rlift00 in hpB.
+        apply hpB.
+      }
+      destruct hpi as [qpi hpi].
+      (* Finally we translate the right Pi1 to put it in the left Sum *)
+      rename e into eA.
+      pose (e := sHeqTypeEq (B2' {0 := sPi1 A2' B2' tp2}) (B1' {0 := sPi1 A1' B1' p1'}) (sHeqSym qpi)).
+      pose (tpi := sTransport (B2' {0 := sPi1 A2' B2' tp2}) (B1' {0 := sPi1 A1' B1' p1'}) e (sPi2 A2' B2' tp2)).
+      (* We conclude *)
+      exists (B1'{ 0 := sPi1 A1' B1' p1' }), (B1'{ 0 := sPi1 A1' B1' p1' }).
+      exists (sPi2 A1' B1' p1'), tpi.
+      exists (sHeqTrans qpi (sHeqTransport e (sPi2 A2' B2' tp2))).
+      destruct hp1' as [[[? ?] ?] ?].
+      destruct htp2 as [[[? ?] ?] ?].
+      destruct hA1' as [[[? ?] ?] ?].
+      destruct hA2' as [[[? ?] ?] ?].
+      destruct hB1' as [[[? ?] ?] ?].
+      destruct hB2' as [[[? ?] ?] ?].
+      repeat split.
+      * assumption.
+      * apply inrel_subst ; try assumption.
+        constructor ; assumption.
+      * apply inrel_subst ; try assumption.
+        constructor ; assumption.
+      * constructor ; assumption.
+      * constructor. constructor ; assumption.
+      * eapply type_HeqTrans' ; try eassumption.
+        eapply type_HeqTransport' ; try assumption.
+        -- eapply type_Pi2' ; eassumption.
+        -- eapply type_HeqTypeEq' ; try assumption.
+           ++ eapply type_HeqSym' ; eassumption.
+           ++ lift_sort. eapply typing_subst ; try eassumption.
+              eapply type_Pi1' ; eassumption.
 
     (* cong_Eq *)
     + destruct (H _ hΓ)
