Translation/XTyping.v
@@ -144,16 +144,24 @@ with eq_term (Σ : sglobal_context) : scontext -> sterm -> sterm -> sterm -> Typ
     Σ ;;; Γ ,, A2 |-x B2 : sSort s2 ->
     Σ ;;; Γ |-x (sSum n1 A1 B1) = (sSum n2 A2 B2) : sSort (max_sort s1 s2)
 
-| cong_Pi1 Γ n A1 A2 B1 B2 s1 s2 p1 p2 :
-    Σ ;;; Γ |-x p1 = p2 : sSum n A1 B1 ->
+| cong_Pi1 Γ nx ny A1 A2 B1 B2 s1 s2 p1 p2 :
+    Σ ;;; Γ |-x p1 = p2 : sSum nx A1 B1 ->
     Σ ;;; Γ |-x A1 = A2 : sSort s1 ->
     Σ ;;; Γ ,, A1 |-x B1 = B2 : sSort s2 ->
+    Σ ;;; Γ ,, A1 |-x B1 : sSort s2 ->
+    Σ ;;; Γ ,, A2 |-x B2 : sSort s2 ->
+    Σ ;;; Γ |-x p1 : sSum nx A1 B1 ->
+    Σ ;;; Γ |-x p2 : sSum ny A2 B2 ->
     Σ ;;; Γ |-x sPi1 A1 B1 p1 = sPi1 A2 B2 p2 : A1
 
-| cong_Pi2 Γ n A1 A2 B1 B2 s1 s2 p1 p2 :
-    Σ ;;; Γ |-x p1 = p2 : sSum n A1 B1 ->
+| cong_Pi2 Γ nx ny A1 A2 B1 B2 s1 s2 p1 p2 :
+    Σ ;;; Γ |-x p1 = p2 : sSum nx A1 B1 ->
     Σ ;;; Γ |-x A1 = A2 : sSort s1 ->
     Σ ;;; Γ ,, A1 |-x B1 = B2 : sSort s2 ->
+    Σ ;;; Γ ,, A1 |-x B1 : sSort s2 ->
+    Σ ;;; Γ ,, A2 |-x B2 : sSort s2 ->
+    Σ ;;; Γ |-x p1 : sSum nx A1 B1 ->
+    Σ ;;; Γ |-x p2 : sSum ny A2 B2 ->
     Σ ;;; Γ |-x sPi2 A1 B1 p1 = sPi2 A2 B2 p2 : B1{ 0 := sPi1 A1 B1 p1 }
 
 | cong_Eq Γ s A1 A2 u1 u2 v1 v2 :
